started refactoring using image functio for expr functions

HM_Theorems.thy
@@ -1,9 +1,9 @@
 theory HM_Theorems
-imports Main HML_list
+imports Main HML_list HML_equivalences
 begin
 
 context lts
-begin
+begin     
 
 section \<open>Hennessy-Milner Theorem of the Trace Modal Logic subset and Trace-equivalence\<close>
 
@@ -46,17 +46,8 @@ next
 qed
 
 lemma ttf_in_HML_trace:
-  fixes t
   shows "(trace_to_formula t) \<in> HML_trace_formulas"
- proof(induction t)
-  case Nil
-  then show ?case 
-    by (simp add: HML_trace_formulas_def trace_conj)
-next
-  case (Cons a t)
-  then show ?case
-    by (simp add: HML_trace_formulas_def trace_pos)
-qed
+  by ((induction t), (simp add: HML_trace_formulas_def trace_conj trace_pos)+)
 
 lemma HM_trace_aux_theorem:
   fixes p \<phi>
@@ -81,34 +72,28 @@ next
 qed
 
 lemma state_satisfies_trace:
-  fixes p t
   assumes "t \<in> traces p"
   shows "p \<Turnstile> trace_to_formula t"
   using \<open>t \<in> traces p\<close>
-proof(induction t arbitrary: p)
-  case Nil
-  then show ?case
-    by simp
-next
-  case (Cons a t)
-  with trace_to_formula.simps(2) show ?case
-    by (smt (verit, best) formula_list.distinct(1) list.inject local.HML_sem_poss mem_Collect_eq step_sequence.cases trace_to_formula.simps(1))
-qed
+  by ((induction t arbitrary: p), simp, 
+(smt (verit, best) formula_list.distinct(1) list.inject local.HML_sem_poss mem_Collect_eq step_sequence.cases trace_to_formula.simps(1, 2)))
 
 text \<open>HM Theorem for Traces\<close>
 
 lemma HM_trace_theorem:
   fixes p q
   shows "(traces p = traces q) = 
-(\<forall>\<phi>. \<phi> \<in> HML_trace_formulas \<longrightarrow> (p \<Turnstile> \<phi> \<longleftrightarrow> q \<Turnstile> \<phi>))"
+HML_trace_equivalent p q"
 proof
   assume trace_eq: "traces p = traces q"
-  show "\<forall>\<phi>. \<phi> \<in> HML_trace_formulas \<longrightarrow> (p \<Turnstile> \<phi>) = (q \<Turnstile> \<phi>)"
-    using HM_trace_aux_theorem state_satisfies_trace trace_eq by blast
+  show "HML_trace_equivalent p q"
+    unfolding HML_trace_equivalent_def using HM_trace_aux_theorem state_satisfies_trace trace_eq 
+    by blast
 next
-  assume assm: "(\<forall>\<phi>. \<phi> \<in> HML_trace_formulas \<longrightarrow> (p \<Turnstile> \<phi> \<longleftrightarrow> q \<Turnstile> \<phi>))"
-  show "traces p = traces q"
-    using state_satisfies_trace assm ttf ttf_in_HML_trace by blast
+  assume assm: "HML_trace_equivalent p q"
+  then show "traces p = traces q"
+    unfolding HML_trace_equivalent_def using state_satisfies_trace assm ttf ttf_in_HML_trace 
+    by blast
 qed
 
 section \<open>Hennessy–Milner Theorem of Modal Logic an Bisimilarity\<close>
@@ -130,75 +115,76 @@ next
     by (metis bisim_sim local.HML_sem_poss)
 qed
 
-function set_to_list2 :: "'b set \<Rightarrow> 'b list" where
-"set_to_list2 s = (if finite s then (if s = {} then [] else 
-                   let x = SOME x. x \<in> s; 
-                    s' = s - {x} in x # set_to_list2 s') else [])"
-  by simp+
 
-termination set_to_list2
-proof
-  show "wf (measure card)"
-    by blast
-  show "\<And>s x xa. finite s \<Longrightarrow> s \<noteq> {} \<Longrightarrow> x = (SOME x. x \<in> s) \<Longrightarrow> xa = s - {x} \<Longrightarrow> (xa, s) \<in> measure card"
-    by (metis card_Diff1_less_iff ex_in_conv in_measure tfl_some)
-qed
+definition set_to_list :: "'s set \<Rightarrow> 's list"
+where \<open>set_to_list s \<equiv> (SOME l. (set l) = s)\<close>
 
+lemma set_to_list_eq:
+  assumes \<open>finite s\<close>
+  shows \<open>set (set_to_list s) = s\<close>
+  unfolding set_to_list_def
+  using someI_ex[OF finite_list[OF assms]] .
 
-lemma 
-  assumes "finite s"
-  defines "s_lst \<equiv> set_to_list2 s"
-  shows "\<forall>x \<in> set s_lst. x \<in> s"
-  using assms
-proof(induction s_lst  arbitrary: s rule: list.induct)
-  case Nil
-  then show ?case by simp
-next
-  case (Cons a s_lst)
-  then have 1: "\<forall>x\<in>set s_lst. x \<in> s" using set_to_list2.simps
-    by (metis DiffE ex_in_conv list.distinct(1) list.inject list.set(1))
-  from Cons(3) have "a = (SOME x. x \<in> s)" using set_to_list2.elims
-    by (metis list.distinct(1) list.sel(1))
-  then have "a \<in> s" 
-    using Cons.hyps(3) some_in_eq by fastforce
-  with 1 show ?case
-    by simp
-qed
-
-function set_to_list :: "'s set \<Rightarrow> 's list" where
-  "set_to_list s = (if finite s then (if s = {} then [] else 
-                   let x = SOME x. x \<in> s; 
-                    s' = s - {x} in x # set_to_list s') else [])"
-  by simp+
-
-termination set_to_list
-proof
-  show "wf (measure card)"
-    by blast
-  show "\<And>s x xa. finite s \<Longrightarrow> s \<noteq> {} \<Longrightarrow> x = (SOME x. x \<in> s) \<Longrightarrow> xa = s - {x} \<Longrightarrow> (xa, s) \<in> measure card"
-    by (metis card_Diff1_less_iff ex_in_conv in_measure tfl_some)
-qed
-
-lemma test:
-  fixes p a
-  defines "der \<equiv> (derivatives p a)"
-  assumes "finite (der)"
-  shows "\<forall>p' \<in> set (set_to_list (der)). p' \<in> der"
+lemma map_SOME:
+  assumes "\<forall>q' \<in> set der_list. \<exists>\<phi>. distinguishes \<phi> p' q'"
+  shows "\<forall>\<psi> \<in> set (map (\<lambda>q'. SOME \<psi>. distinguishes \<psi> p' q') der_list). p' \<Turnstile> \<psi>"
 proof-
-  define der_lst where "der_lst \<equiv> set_to_list (der)"
-  then show "\<forall>p'\<in>set (set_to_list der). p' \<in> der"
-  using assms(2)
-proof(induction der_lst arbitrary: der rule: list.induct)
-  case Nil
-  then show ?case by simp
-next
-  case (Cons hd rest)
-  then have 1: "\<forall>x\<in>set rest. x \<in> der" unfolding der_lst_def der_def using set_to_list.simps
-    by (metis finite_Diff insert_Diff insert_iff list.distinct(1) list.sel(3) some_in_eq)
-  from Cons(3) have "hd \<in> der" using some_in_eq set_to_list.elims 
-    by (metis Cons.hyps(2) list.distinct(1) list.sel(1))
-  with 1 show ?case
-    by (metis Cons.hyps(2) set_ConsD)
+  define \<psi>_list where "\<psi>_list \<equiv> (map (\<lambda>q'. SOME \<psi>. distinguishes \<psi> p' q') der_list)"
+  then show "\<forall>\<psi> \<in> set \<psi>_list. p' \<Turnstile> \<psi>"
+    using assms
+  proof(induction \<psi>_list arbitrary: der_list)
+    case Nil
+    then show ?case
+      by fastforce
+  next
+    case (Cons a \<psi>_tail) 
+    have \<psi>_head: "\<exists>\<phi>. distinguishes \<phi> p' (hd der_list)"
+      using local.Cons(2, 3) by force
+    then have dist: "distinguishes (SOME \<phi>. distinguishes \<phi> p' (hd der_list)) p' (hd der_list)"
+      using someI_ex
+      by (metis (no_types, lifting))
+    from Cons(3) have a_eq: "a = (SOME \<psi>. distinguishes \<psi> p' (hd der_list))"
+      using Cons.hyps(2) by force
+    with dist have a_dist: "distinguishes a p' (hd der_list)"
+      by blast
+    from Cons have "\<forall>\<psi>\<in>set \<psi>_tail. p' \<Turnstile> \<psi>"
+      by auto
+    with a_eq a_dist show ?case
+      by simp
+  qed
+qed
+
+lemma dinst_junctor_implies_dist_conjunction:
+  assumes "\<forall>q' \<in> set der_list. \<exists>\<phi>. distinguishes \<phi> p' q'"
+  shows "(\<forall>q' \<in> set der_list. \<not>q' \<Turnstile> HML_conj (map (\<lambda>q'. SOME \<psi>. distinguishes \<psi> p' q') der_list) [])"
+proof
+  fix q'
+  assume q'_fix: "q' \<in> set der_list"
+  define \<psi>d_list where \<open>\<psi>d_list \<equiv> (map (\<lambda>q'. SOME \<psi>. distinguishes \<psi> p' q') der_list)\<close>
+  then show "(\<not>q' \<Turnstile> HML_conj \<psi>d_list [])"
+    using assms q'_fix
+  proof(induction der_list arbitrary: \<psi>d_list)
+    case Nil
+    then show ?case
+      by force
+  next
+    case (Cons a \<psi>d_list)
+    from Cons(3) have "q' = a \<or> q' \<in> set \<psi>d_list"
+      by auto
+    then show ?case
+    proof
+      assume "q' = a"
+      with Cons obtain \<phi> where "distinguishes \<phi> p' q'"
+        by fastforce
+      thus ?thesis using \<open>q' = a\<close> Cons(2) someI_ex HML_sem_conj
+        by (metis (no_types, lifting) list.set_intros(1) list.simps(9))
+    next
+      assume "q' \<in> set \<psi>d_list"
+      with Cons have "\<not> q' \<Turnstile> HML_conj (map (\<lambda>q'. SOME \<psi>. distinguishes \<psi> p' q') \<psi>d_list) []"
+        by simp
+      then show ?thesis
+        by auto
+    qed
   qed
 qed
 
@@ -211,67 +197,30 @@ proof (safe, rule ccontr)
   define der where \<open>der \<equiv> derivatives q a\<close>
   define der_list where \<open>der_list \<equiv> set_to_list der\<close>
   from assms have "finite der" unfolding image_finite_def der_def by simp
-  with der_list_def have "\<forall>q' \<in> set der_list. q' \<in> der"
-  proof(induction der_list arbitrary: der)
-    case Nil
-    then show ?case by simp
-  next
-    case (Cons hd rest)
-    from Cons have "\<forall>q'\<in>set rest. q' \<in> der" unfolding der_list_def der_def using set_to_list.simps  
-    by (metis finite_Diff insert_Diff insert_iff list.distinct(1) list.sel(3) some_in_eq)
-    then show ?case using some_in_eq set_to_list.elims 
-      by (metis Cons.hyps(2) list.distinct(1) list.inject set_ConsD)
-  qed
+  with set_to_list_eq have "\<forall>q' \<in> set der_list. q' \<in> der" unfolding der_list_def der_def set_to_list_def
+    by blast
   define \<phi>d_list where \<open>\<phi>d_list \<equiv> map (\<lambda>q'. SOME \<psi>. distinguishes \<psi> p' q') der_list\<close>
   define \<phi>d where \<open>\<phi>d \<equiv> HML_poss a (HML_conj \<phi>d_list [])\<close>
   assume contra_assms:
     \<open>p \<mapsto> a p'\<close> \<open>HML_equivalent p q\<close> \<open>\<nexists>q'. q \<mapsto> a q' \<and>  HML_equivalent p' q'\<close>
   hence dist_exists: \<open>\<forall>q' \<in> der. \<exists>\<phi>. distinguishes \<phi> p' q'\<close>
     unfolding der_def using hml_distinctions by simp
-  then have dist: "\<forall>q' \<in> set (set_to_list der). \<exists>\<phi>. distinguishes \<phi> p' q'"
+  hence dist: "\<forall>q' \<in> set (set_to_list der). \<exists>\<phi>. distinguishes \<phi> p' q'"
     using \<open>\<forall>q'\<in>set der_list. q' \<in> der\<close> der_list_def by blast
   hence "\<forall>\<psi> \<in> set \<phi>d_list. p' \<Turnstile> \<psi>"
-    unfolding \<phi>d_list_def  
-    using der_list_def
-  proof(induction der_list arbitrary: der rule: list.induct)
-    case Nil
-    then show ?case by simp 
-  next
-    case (Cons hd tail)
-    then have A1: "tail = set_to_list (der - {hd})" using set_to_list.elims 
-      by (metis (no_types, lifting) list.discI list.inject)
-    with Cons have A2: " \<forall>q'\<in>set (set_to_list (der - {hd})). \<exists>\<phi>. distinguishes \<phi> p' q'" 
-      using set_to_list.elims 
-      by (metis list.set_intros(2))
-    with A1 Cons have 1: "\<forall>a\<in>set (map (\<lambda>q'. SOME \<psi>. distinguishes \<psi> p' q') tail). p' \<Turnstile> a" 
-      by blast
-    from Cons have "\<exists>\<psi>. distinguishes \<psi> p' hd" using der_list_def set_to_list.simps
-      by (metis list.set_intros(1))
-    then have "p' \<Turnstile> (SOME \<psi>. distinguishes \<psi> p' hd)" 
-      by (metis (mono_tags, lifting) someI2_ex)
-    with 1 show ?case 
-      by (metis (no_types, lifting) list.simps(9) set_ConsD) 
-  qed
-  hence p'_sat: "p' \<Turnstile> (HML_conj \<phi>d_list [])" 
-    by force
+    using map_SOME
+    unfolding \<phi>d_list_def der_list_def
+    by blast
+  hence p'_sat: "p' \<Turnstile> (HML_conj \<phi>d_list [])"
+    using HML_semantics.simps(1) by simp
   with contra_assms(1) have "p \<Turnstile> \<phi>d" unfolding \<phi>d_def
     using local.HML_sem_poss by blast
-  have \<open>(\<forall>q'. q' \<in> der \<longrightarrow> \<not>q' \<Turnstile> HML_conj \<phi>d_list [])\<close>
-  proof safe
-    fix q'
-    assume q'_in_der: "q' \<in> der" and q'_sat: "q' \<Turnstile> HML_conj \<phi>d_list []"
-    from dist_exists have "\<exists>\<phi>. distinguishes \<phi> p' q'"
-      using q'_in_der by blast
-    from q'_in_der have "q \<mapsto>a q'" unfolding der_def
-      by blast
-    with contra_assms(3) have "\<not>(\<forall> \<phi>::('a) formula_list. (p' \<Turnstile> \<phi>) \<longrightarrow> (q' \<Turnstile> \<phi>))" 
-      unfolding HML_equivalent_def
-      using \<open>\<exists>\<phi>. distinguishes \<phi> p' q'\<close> by blast
-    with contra_assms equiv_der show False
-      using \<open>q \<mapsto>a q'\<close> by blast
-  qed
+  have \<open>(\<forall>q' \<in> der. \<not>q' \<Turnstile> HML_conj \<phi>d_list [])\<close> 
+    using dinst_junctor_implies_dist_conjunction dist_exists
+    unfolding \<phi>d_list_def der_def
+    using \<open>finite der\<close> der_def der_list_def set_to_list_eq by blast
   with contra_assms(1) \<open>p' \<Turnstile> HML_conj \<phi>d_list []\<close> have \<open>distinguishes \<phi>d p q\<close>
-    using \<phi>d_def der_def by auto
+    unfolding \<phi>d_def der_def by auto
   thus False using contra_assms unfolding HML_equivalent_def by blast
 qed
 
@@ -283,7 +232,15 @@ theorem Hennessy_Milner_theorem:
   unfolding bisimilar_def HML_equivalent_def
   using assms by blast
 
+theorem HM_simulation_theorem:
+  assumes "image_finite"
+  shows "HML_simulation_equivalent p q = (p \<simeq>F q)"
+  oops
 
+theorem HM_possible_futures_theorem:
+  assumes "image_finite"
+  shows "HML_possible_futures_equivalent p q = (p \<simeq>PF q)"
+  oops
 
 end
 end
