HML_equivalences.thy
@@ -1,0 +1,19 @@
+theory HML_equivalences
+imports Main
+HML_list
+begin
+
+context lts begin
+
+definition HML_trace_equivalent where
+"HML_trace_equivalent p q \<equiv> (\<forall> \<phi>. \<phi> \<in> HML_trace_formulas \<longrightarrow> (p \<Turnstile> \<phi>) \<longleftrightarrow> (q \<Turnstile> \<phi>))"
+
+definition HML_simulation_equivalent :: \<open>'s \<Rightarrow> 's \<Rightarrow> bool\<close> where
+  "HML_simulation_equivalent p q \<equiv> 
+(\<forall>\<phi>. \<phi> \<in> HML_simulation_formulas \<longrightarrow> (p \<Turnstile> \<phi> \<longleftrightarrow> q \<Turnstile> \<phi>))"
+
+definition HML_possible_futures_equivalent where
+"HML_possible_futures_equivalent p q \<equiv> (\<forall> \<phi>. \<phi> \<in> HML_possible_futures_formulas \<longrightarrow> (p \<Turnstile> \<phi>) \<longleftrightarrow> (q \<Turnstile> \<phi>))"
+
+end
+end
